# baseURI: https://linked.data.gov.au/def/irg
# imports: http://purl.org/dc/terms/
# imports: http://purl.org/linked-data/registry
# imports: http://purl.org/linked-data/version
# imports: http://www.w3.org/2006/time
# imports: http://xmlns.com/foaf/spec/
# prefix: irg

@prefix dcterms: <http://purl.org/dc/terms/> .
@prefix irg: <https://linked.data.gov.au/def/irg#> .
@prefix owl: <http://www.w3.org/2002/07/owl#> .
@prefix rdf: <http://www.w3.org/1999/02/22-rdf-syntax-ns#> .
@prefix rdfs: <http://www.w3.org/2000/01/rdf-schema#> .
@prefix reg: <http://purl.org/linked-data/registry#> .
@prefix skos: <http://www.w3.org/2004/02/skos/core#> .
@prefix time: <http://www.w3.org/2006/time#> .
@prefix xsd: <http://www.w3.org/2001/XMLSchema#> .

<https://linked.data.gov.au/def/irg>
  a owl:Ontology ;
  rdfs:comment """This ontology is a specialisation of the [Registry Ontology](http://purl.org/linked-data/registry) (REG) used to manage Internationalized Resource Identifiers (IRIs). \"IRI\" is a generalised and more modern name for URIs - Uniform Resource Identifiers.

The major specialisation in this ontology is the subclassing of reg:RegisterItem to `irg:RegisteredIRI` which just mandates the use of a few extra properties for IRI management.

Another difference between this ontology and REG is not IRI-specific but a general development: here we define the statuses of `reg:RegisterItem` instances to be held within temporal objects, `irg:StatusPeriod` instances, sub classes of OWL TIME's `time:ProperInterval` allowing us to stack up multiple, time-bounded, statuses per `irg:RegisteredIRI`."""@en ;
  rdfs:label "IRI Registry Ontology" ;
  owl:imports dcterms: ;
  owl:imports <http://purl.org/linked-data/registry> ;
  owl:imports <http://purl.org/linked-data/version> ;
  owl:imports <http://www.w3.org/2006/time> ;
  owl:imports <http://xmlns.com/foaf/spec/> ;
.
irg:IRIOwner
  a owl:Class ;
  rdfs:comment """An IRI Owner is an Organisation that is requesting, or has requested, an IRI allocation within the IRI Registry.

IRI Owners need to have a specific person play the role of Submitter to actually make the submission.

The rules governing eligibility of Organisations to be IRI Owners for the 'AGLDWG IRI Register' are described in the AGLDWG's Guidelines document, see <https://linked.data.gov.au/guidelines>."""@en ;
  rdfs:label "IRI Owner" ;
  rdfs:subClassOf <http://xmlns.com/foaf/0.1/Organization> ;
.
irg:IRIRedirectTestCase
  a owl:Class ;
  rdfs:comment "An IRI Redirect Test Case is an object used to contain the inputs and outputs needed to test the functioning of IRI redirects."@en ;
  rdfs:label "IRI Redirect Test Case" ;
  rdfs:subClassOf owl:Thing ;
.
irg:IRIRegister
  a owl:Class ;
  rdfs:comment "An IRI Register is a Registry Ontology Register used to manage IRIs. For this reason, it has restrictions (requirements) on several properties not present in the Registry Ontology needed to manage IRIs."@en ;
  rdfs:label "IRI Register" ;
  rdfs:subClassOf reg:Register ;
.
irg:IRIResourceType
  a owl:Class ;
  rdfs:comment """An IRI Resource Type is a type of Resource for which a Registered IRI can be allocated.

Examples of IRI Resource Types include: Definitional Item, Dataset, Top-level Register, Second-level Register"""@en ;
  rdfs:label "IRI Resource Type" ;
  rdfs:subClassOf skos:Concept ;
.
irg:IRISubmitter
  a rdfs:Class ;
  a owl:Class ;
  rdfs:comment "An IRI Submitter is a Person that requests an IRI to be allocated within an IRI Registry and does so on behalf of an IRI Owner, which is an Organisation entitled to have IRIs allocated."@en ;
  rdfs:label "IRI Submitter" ;
  rdfs:subClassOf <http://xmlns.com/foaf/0.1/Person> ;
.
irg:RegisteredIRI
  a owl:Class ;
  rdfs:comment """A Registered Item that is for an IRI.

It is expected that only IRIs are registered using this class and that the IRI registered is indicated using the property irg:forIRI."""@en ;
  rdfs:label "Registered IRI" ;
  rdfs:subClassOf reg:RegisterItem ;
  rdfs:subClassOf [
      a owl:Restriction ;
      owl:cardinality "1"^^xsd:nonNegativeInteger ;
      owl:onProperty irg:forIRI ;
    ] ;
  rdfs:subClassOf [
      a owl:Restriction ;
      owl:cardinality "1"^^xsd:nonNegativeInteger ;
      owl:onProperty irg:hasIriRedirectCode ;
    ] ;
  rdfs:subClassOf [
      a owl:Restriction ;
      owl:cardinality "1"^^xsd:nonNegativeInteger ;
      owl:onProperty irg:hasIriResourceType ;
    ] ;
  rdfs:subClassOf [
      a owl:Restriction ;
      owl:cardinality "1"^^xsd:nonNegativeInteger ;
      owl:onProperty irg:hasIriSubmitter ;
    ] ;
  rdfs:subClassOf [
      a owl:Restriction ;      
      owl:cardinality "1"^^xsd:nonNegativeInteger ;
      owl:onProperty reg:owner; 
  ];
.
irg:actsFor
  a owl:ObjectProperty ;
  rdfs:comment "This property is used to indicate the Government Organisation that an IRI Submitter is requesting IRI allocations for."@en ;
  rdfs:domain irg:IRISubmitter ;
  rdfs:label "acts for" ;
  rdfs:range irg:IRIOwner ;
.
irg:agldwgIriRegister
  a irg:IRIRegister ;
  reg:manager <https://linked.data.gov.au/org/agldwg> ;
  reg:owner <https://linked.data.gov.au/org/agldwg> ;
  rdfs:comment """This particular Register is the Register used by the Australian Government Linked Data Working Group (AGLDWG - see https://www.linked.data.gov.au) to register IRIs using the linked.data.gov.au domain.

IRIs allocated in this domain are intended for use with Linked Data data and applications and are allocated for Australian governments' purposes."""@en ;
  rdfs:label "AGLDWG IRI Register" ;
.
irg:dataset
  a irg:IRIResourceType ;
  dcterms:source "The AGLDWG's Guidelines, see <https://www.linked.data.gov.au/guidelines>" ;
  rdfs:comment "The type of IRI Resource for which IRIs containing /dataset/ are allocated."@en ;
  rdfs:label "Dataset" ;
.
irg:definitionalItem
  a irg:IRIResourceType ;
  dcterms:source "The AGLDWG's Guidelines, see <https://www.linked.data.gov.au/guidelines>" ;
  rdfs:comment "The type of IRI Resource for which IRIs containing /def/ are allocated."@en ;
  rdfs:label "Definitional Item" ;
.
irg:forIRI
  a owl:AnnotationProperty ;
  rdfs:comment "This property indicates the thing for which the Registered IRI instance has been created - the IRI that is registered."@en ;
  rdfs:domain irg:RegisteredIRI ;
  rdfs:label "for IRI" ;
  rdfs:range xsd:anyURI ;
.
irg:fromIRI
  a owl:DatatypeProperty ;
  rdfs:comment "This property indicates the input/source IRI that a test case redirect from, to some other IRI."@en ;
  rdfs:domain irg:IRIRedirectTestCase ;
  rdfs:label "from IRI" ;
  rdfs:range xsd:anyURI ;
.
irg:hasHttpResponseHeaders
  a owl:DatatypeProperty ;
  rdfs:comment "This property indicates any HTTP headers that need to be returned by the redirect service for a successful result in the testing of this Test Case."@en ;
  rdfs:domain irg:IRIRedirectTestCase ;
  rdfs:label "HTTP Response Headers" ;
  rdfs:range xsd:string ;
.
irg:hasHttpReqestHeaders
  a owl:DatatypeProperty ;
  rdfs:comment "This property indicates any HTTP headers that need to be submitted with the HTTP request to trigger the redirect being testedby this Test Case."@en ;
  rdfs:domain irg:IRIRedirectTestCase ;
  rdfs:label "HTTP Request Headers" ;
  rdfs:range xsd:string ;
.
irg:hasIriRedirectCode
  a owl:AnnotationProperty ;
  rdfs:comment """This property indicates the code used to redirect the registered IRI to the functional data or system IRIs.

Expected values for this property are XSD strings that contain Apache2 mod_rewrite, nginx or similar code."""@en ;
  rdfs:label "has IRI redirect code" ;
  rdfs:range xsd:string ;
  skos:example """# IRI for the AGRIF Ontology, http://linked.data.gov.au/def/agrif
# Apache mod_rewrite
RewriteCond %{QUERY_STRING} ^_format=text/turtle$ [OR]
RewriteCond %{HTTP:Accept} text/turtle [NC]
RewriteRule ^/def/agrif(.*)$        https://raw.githack.com/agldwg/agrif-ont/master/agrif.ttl? [R=302,L]
RewriteRule ^/def/agrif(.*).ttl$    https://raw.githack.com/agldwg/agrif-ont/master/agrif.ttl [R=302,L]
RewriteRule ^/def/agrif(.*)$        https://raw.githack.com/agldwg/agrif-ont/master/agrif.html$1 [R=302,L]""" ;
.
irg:hasIriResourceType
  a owl:ObjectProperty ;
  rdfs:comment "This property indicates one of the IRI Resource Types, listed within this ontology, that a RegisteredIRI is allocated for."@en ;
  rdfs:domain irg:RegisteredIRI ;
  rdfs:label "IRI resource type" ;
  rdfs:range irg:IRIResourceType ;
  rdfs:subPropertyOf dcterms:type ;
.
irg:hasIriSubmitter
  a owl:ObjectProperty ;
  rdfs:comment "This property indicates an IRI Submitter Agent that is or has requested IRIs within the AGLDWG IRI Register."@en ;
  rdfs:label "has IRI submitter" ;
  rdfs:range irg:IRIOwner ;
  rdfs:subPropertyOf reg:submitter ;
.
irg:secondLevelRegister
  a irg:IRIResourceType ;
  dcterms:source "The AGLDWG's Guidelines, see <https://www.linked.data.gov.au/guidelines>" ;
  rdfs:comment "The type of IRI Resource for which modularised subregisters of a Top-Level Register or subregisters of a Dataset are allocated."@en ;
  rdfs:label "Second-Level Register" ;
.
irg:toIRI
  a owl:DatatypeProperty ;
  rdfs:comment "This property indicates the output/destination IRI that a Test Case redirect to, from some other IRI."@en ;
  rdfs:domain irg:IRIRedirectTestCase ;
  rdfs:label "to IRI" ;
  rdfs:range xsd:anyURI ;
.
irg:topLevelRegister
  a irg:IRIResourceType ;
  dcterms:source "The AGLDWG's Guidelines, see <https://www.linked.data.gov.au/guidelines>" ;
  rdfs:comment "The type of IRI Resource for which IRIs containing a to-level path segment after the PID domain are allocated."@en ;
  rdfs:label "Top-Level Register" ;
.
